---
title: "Engineering Mathematics I"
subtitle: '<font color="red">Chapter 4. The Laplace Transform</font>'
format:
  revealjs: 
    slide-level: 3
    slide-number: true
    smaller: false
    chalkboard: 
      buttons: true
    preview-links: auto
    logo: images/seoultech_logo.png
    css: styles.css
    pointer:
      pointerSize: 20
      color: '#32cd32'
revealjs-plugins:
  - pointer 
  - confetti
filters:
  - reveal-header
  - code-fullscreen     
jupyter: python3    
---

### 4.1 Definition of the Laplace Transform

-  If $f$ be a function defined for $t \geq 0$, $~$then the *integral*

   <font color='red'>$$\mathcal{L}\{f(t)\} =\int_0^\infty f(t) e^{-st}\, dt =F(s)$$</font>

   is the **Laplace Transform** of $~f$ provided the integral converges. The result is a function of $s$
 
---

 **Example:** $~$ Evaluate $\mathcal{L}\{1\}$, $~\mathcal{L}\{t\}$, $~$and $~\mathcal{L}\{e^{-3t}\}$

---

**Example:** $~$ Evaluate $\mathcal{L}\{f(t)\}~$ for $~\displaystyle f(t) = \left\{\begin{matrix}
0, & 0 \leq  t < 3\\ 
2, & \;\;\;\;\;t \geq 3
\end{matrix}\right.$

---

* $\mathcal{L}$ is a linear transform

$$\mathcal{L}\{\alpha f(t) +\beta g(t)\} = \alpha \mathcal{L} \{f(t)\} +\beta\mathcal{L}\{g(t)\} =\alpha F(s) +\beta G(s)$$

---

**Example:** $~$ Find $\mathcal{L}\{f(t)\}$ by first using an appropriate trigonometric identity $~f(t)=\sin^2 2t$

---

**Example:** $~$ Find $\mathcal{L}\{f(t)\}$

-  $~f(t)=\left\{\begin{matrix}
 -1,& 0 \leq t < 1\\ 
 1,& t \geq 1\;\;\;\;\;\;\,
\end{matrix}\right.$

<br/>

. . .

-  $~f(t)=\left\{\begin{matrix}
 t,& 0 \leq t < 1\\ 
 1,& t \geq 1\;\;\;\;\,
\end{matrix}\right.$

<br/>

. . .

-  $~f(t)=\left\{\begin{matrix}
 \sin t,& 0 \leq t < \pi\\ 
 0,& t \geq \pi\;\;\;\;\;\,
\end{matrix}\right.$

---

**Example:** $~$ Find $\mathcal{L}\{f(t)\}$

-  $~f(t)=e^{t+7}$

. . .

-  $~f(t)=e^t \cos t$

. . .

-  $~f(t)=t\cos t$

. . .

-  $~f(t)=\sin 3t \cos 3t$

. . .

-  $~f(t)=\sin^4 t$

### 4.2 The Inverse Transform and Transforms of Derivatives

::: {.incremental}
-  If $F(s)$ represents the Laplace transform of $~f(t)$, $~$then $f(t)$ is the **inverse Laplace transform** of $F(s)$

   $$f(t)=\mathcal{L}^{-1}\{F(s)\}$$
  
-  $\mathcal{L}^{-1}$ is a linear transform

   $$\mathcal{L}^{-1}\{\alpha F(s) +\beta G(s)\} = \alpha \mathcal{L}^{-1} \{F(s)\} +\beta\mathcal{L}^{-1}\{G(s)\} =\alpha f(t) +\beta g(t)$$
:::
--- 

**Example:** $~$ Evaluate $\displaystyle\mathcal{L}^{-1}\left\{\frac{-2s +6}{s^2 +4}\right\}$

---

-  **Transforms of derivatives**

   $$\begin{align*}
    \mathcal{L}\{f'(t)\} &= sF(s) -f(0)\\ 
    \mathcal{L}\{f''(t)\} &= s^2F(s) -sf(0) -f'(0)\\ 
    &\; \vdots  
   \end{align*}$$
  
   $\displaystyle\mathcal{L}\left\{\frac{d^n f}{dt^n}\right\}$ depends on $F(s)=\mathcal{L}\{f(t)\}$ and the $n-1$ derivatives of $~f(t)$ evaluated at $t=0$
  
---  

-  If $~f$ is piecewise continuous on $[0, \infty]$ and of exponential order, then

   $$\lim_{s \to \infty} \mathcal{L}\{f(t)\}=0$$

. . .

-  The Laplace transform of a linear DE with constant coefficients becomes an algebraic equation in $Y(s)$

. . .

**Example:** $~$ Use the Laplace transform to solve the IVP
  
 $$\frac{dy}{dt} +3y = 13\sin 2t, \;y(0)=6$$  

 ---

**Example:** $~$  Find the given inverse transform

::: columns

:::{.column width=50%}
:::{.incremental}
-  $\displaystyle \mathcal{L}^{-1} \left\{ \frac{1}{s^3} \right\}$

   <br/>

-  $\displaystyle \mathcal{L}^{-1} \left\{ \frac{1}{s^2} - \frac{48}{s^5} \right\}$

   <br/>

-  $\displaystyle \mathcal{L}^{-1} \left\{ \frac{(s+1)^3}{s^4} \right\}$
:::
:::

:::{.column width=50%}
:::{.incremental}
-  $\displaystyle \mathcal{L}^{-1} \left\{ \frac{1}{4s^2+1} \right\}$

   <br/>
  
-  $\displaystyle \mathcal{L}^{-1} \left\{ \frac{s+1}{s^2+2} \right\}$
:::
:::

:::

---

**Example:** $~$  Use the Laplace transform to solve the given initial-value problem

::: {.incremental}
-  $~y''+y=\sqrt{2} \sin \sqrt{2}t, \;\;y(0)=10,\;y'(0)=0$
  
   <br/>
  
-  $~2y'''+3y''-3y'-2y=e^{-t}, \;\;y(0)=0, \;y'(0)=0, \; y''(0)=1$
:::


### 4.3 Translation Theorems

-  **First Translation Theorem**

   If $\mathcal{L}\{f(t)\}=F(s)~$ and $~a$ is any real number, $~$then 
  
   $$\mathcal{L}\{e^{-at}f(t)\}=F(s+a)$$

. . .
  
**Example:** $~$ Evaluate $\mathcal{L}\{e^{-2t}\cos 4t\}$ and $\displaystyle\mathcal{L}^{-1}\left\{\frac{2s +5}{(s +3)^2}\right\}$

---

-  **Second Translation Theorem**

   If $\mathcal{L}\{f(t)\}=F(s)~$ and $~a >0$, then 
  
$$\mathcal{L}\{f(t -a)\mathcal{U}(t -a)\}=e^{-as}F(s)$$

. . .

-  **Alternative Form**
  
   $$\begin{align*}
       \mathcal{L}\{g(t)\mathcal{U}(t -a)\} &= {\scriptsize\int_a^\infty e^{-st} g(t)\,dt}\\ 
        &{\scriptsize = \int_0^\infty e^{-s(t'+a)} g(t' +a) \,dt'} = e^{-as} \mathcal{L}\{g(t+a)\}
   \end{align*}$$

---

**Example:** $~$ Solve $~y' +y = f(t)$, $~$$y(0)=5$, $~$ 

$~$ where 

$$f(t) =
    \begin{cases}
       0, & 0 \leq t < \pi\\ 
       3\cos t ,& t \geq \pi
    \end{cases}$$

---


**Example:** $~$ Find either $~F(s)$ or $~f(t)$

::: columns

::: {.column width="50%"}
::: {.incremental}
-  $\mathcal{L}\{ te^{10t} \}$

   <br/>

-  $\mathcal{L}\{ t^{10}e^{-7t}\}$

   <br/>
  
-  $\mathcal{L}\{ e^t \sin 3t \}$
:::
:::

::: {.column width="50%"}
::: {.incremental}
-  $\displaystyle \mathcal{L}^{-1} \left\{ \frac{s}{(s+1)^2} \right\}$

   <br/>
  
-  $\displaystyle \mathcal{L}^{-1} \left\{ \frac{2s-1}{s^2(s+1)^3} \right\}$
:::
:::

:::


### 4.4 $~$Additional Operational Properties

. . .

-  **Derivatives of Transforms:** $~$ If $F(s)=\mathcal{L}\{f(t)\}~$ and $n=1,2,\cdots$, then

   $$\mathcal{L}\{t^nf(t)\}=(-1)^n \frac{d^n}{ds^n} F(s)$$
  
   **Example:** $~$ Evaluate $~\mathcal{L}\{t\sin \omega t\}$
  
   <br/>
   
   **Example:** $~$ Solve $~x'' +16x =\cos 4t, \; x(0)=1, \; x'(0)=1$

---

- **Convolution Theorem:** $\text{ }$ $\displaystyle f*g=\int_0^t f(\tau)g(t -\tau)\, d\tau$

  $$\mathcal{L}\{f*g\}=\mathcal{L}\{f(t)\} \mathcal{L}\{g(t)\} =F(s) G(s)$$
  
  **Example:** $\text{ }$ Evaluate $\displaystyle\mathcal{L}^{-1}\left\{\frac{1}{(s^2 +\omega^2)^2}\right\}$
  
  **Example:** $\text{ }$ Evaluate $\displaystyle\mathcal{L} \left\{ \int_0^t f(\tau)\, d\tau \right\}$
  
  **Example:** $\text{ }$ Solve $\displaystyle f(t) =3t^2 -e^{-t} -\int_0^t f(\tau)\, e^{t -\tau}\, d\tau\;$ for $f(t)$
---

-  **Transform of a Periodic Function:** $~$ $f(t+T)=f(t)$

   $$\scriptsize\mathcal{L}\{f(t)\}=\frac{1}{1-e^{-sT}} \int_0^T e^{-st} f(t) \,dt$$
  
   **Example:** $~$ Find the Laplace transform of the periodic function
  
   ![](figures/ch04_figure01.png "Square wave"){width="30%" fig-align="center"}
  
   $$\scriptsize\mathcal{L}\{E(t)\}=\frac{1}{1 -e^{-2s}} \int_0^2 e^{-st} E(t)\,dt=\frac{1}{s(1 +e^{-s})}$$

---

**Example:** $~$Evaluate the given Laplace transform

::: {.incremental}
-  $~\mathcal{L}\left\{ te^{-10t} \right\}$
 
   <br/>

-  $~\mathcal{L}\left\{ t\cos 2t \right\}$

   <br/>
  
-  $~\mathcal{L}\left\{ te^{2t}\sin 6t \right\}$
:::

---

**Example:** $~$ Use the Laplace transform to solve the given initial-value problem

::: {.incremental}
-  $~y'+y=t \sin t, \;y(0)=0$
 
   <br/>

-  $~y''+9y=\cos 3t, \;y(0)=2, \;y'(0)=5$

:::

---

**Example:** $~$ Find the convolution $~f*g$ of the given functions. After integrating find the Laplace transform $~f*g$

::: {.incremental}
-  $~f(t)=4t, \;g(t)=3t^2$
 
   <br/>

-  $~f(t)=e^{-t}, \;g(t)=e^t$
 
   <br/>
:::

. . .

**Example:** $~$  Find the Laplace transform

-  $~\mathcal{L} \left\{ e^{-t}* e^t \cos t \right\}$

---

**Example:** $~$  Evaluate the given inverse transform

-  $~\displaystyle \mathcal{L}^{-1} \left\{ \frac{1}{s^3(s-1)} \right\}$

---

**Example:** $~$  Use the Laplace transform  to solve the given integral or integrodifferential equation

::: {.incremental} 
-  $~\displaystyle f(t) +2\int_0^t f(\tau)\cos (t-\tau)\,d\tau=4e^{-t}+\sin t$

   <br/>
  
-  $~\displaystyle \frac{dy}{dt}=10-\int_0^t e^{-4t} y(t-\tau)\,d\tau, \;y(0)=5$
:::

---

**Example:** $~$  The Laplace transform $\mathcal{L} \left\{ e^{-t^2} \right\}$ exists, but without finding it solve the initial-value problem

-  $~y''+9y=3e^{-t^2}, \;\;y(0)=0, \;y'(0)=0$

   <br/>

. . .

**Example:** $~$   Solve the integral equation

-  $~\displaystyle f(t)=e^t+e^t \int_0^t e^{-\tau} f(\tau)\, d\tau$


### 4.5 $~$The Dirac Delta Function

::: columns

::: {.column width=55%}
**Unit Pulse** 
  
$$\scriptsize
     \delta_a(t-t_0) = 
       \left\{\begin{matrix}
          0, & \;\;\;\;\;\; 0 \leq t < t_0 -a\\ 
          \frac{1}{2a}, & t_0 -a \leq t \leq t_0 +a\\ 
          0, & \;\; t \geq t_0 +a
       \end{matrix}\right.$$
:::

::: {.column width=45%}

![](figures/ch04_figure02.png "Dirac delta function"){width="60%" fig-align="center"}

:::

:::   

---

-  **The Dirac Delta Function**
  
   $$\displaystyle
   \begin{align*}
     \delta(t -t_0) &= \lim_{a \to 0} \,\delta_a(t -t_0) \\
     &\Downarrow \\
     \mathcal{L}\{\delta(t -t_0)\} &= \lim_{a \to 0} \mathcal{L}\{\delta_a(t -t_0)\}=e^{-st_0}\lim_{a \to 0} \left(\frac{e^{sa} -e^{-sa}}{2sa}\right)\\ 
     &= e^{-st_0}
   \end{align*}$$
  
   When $~t_0=0$, $~$$\displaystyle\mathcal{L}\{\delta(t)\}=1$

---

**Example:** $~$ Solve $~y'' +y=4\delta(t -2\pi)$ $~$subject to $y(0)=1, \;y'(0)=0$

---

**Example:** $~$ Use the Laplace transform to solve the given differential equation subject to the indicated initial conditions

::: {.incremental}
-  $~y'-3y=\delta(t-2), \;y(0)=0$

   <br/>
  
-  $~y''+y=\delta(t-2\pi), \;y(0)=0, \,y'(0)=1$

   <br/>
  
-  $~y''+y=\delta(t-\pi/2)+\delta(t-3\pi/2),\;y(0)=0,\,y'(0)=0$
:::


### 4.6 $~$ Systems of Linear Differential Equations

When initial conditions are specified, $~$the Laplace transform reduces a system of linear DEs to a set of simultaneous algebraic equations in the transformed functions

<br/>

. . .

**Example:** $~$ Double Pendulum

![](figures/ch04_figure03.png "Double Pendulum"){width="25%" fig-align="center"}

---

**Linearization** $~$ For small displacements $\theta_1$ and $\theta_2$,

$$\begin{align*}
  (m_1 +m_2) l_1 \ddot{\theta_1} +m_2 l_2 \ddot{\theta_2} +(m_1 +m_2) g \,\theta_1 &= 0\\ 
  l_2 \ddot{\theta_2} +l_1 \ddot{\theta_1} +g \,\theta_2 &= 0
\end{align*}$$

<br/>
Solve the system when 

$$m_1=3, m_2=1, l_1=l_2=5, \text{ and } ~g=10$$

$$\theta_1(0) = 1, \theta_2(0)=-1, \dot{\theta_1}(0)=0,  \dot{\theta_2}(0)=0$$

---

**Example:** $~$ Use the Laplace transform to solve the given system of differential equations

$$\begin{align*}
     \dot{x} &= -x+y \\ 
     \dot{y} &= 2x, \;\;x(0)=0,\;y(0)=1 
   \end{align*}$$
   
. . .

$$\begin{align*}
    \dot{x} &= x-2y \\ 
    \dot{y} &= 5x-y, \;\;x(0)=-1,\;y(0)=2 
   \end{align*}$$

. . .

$$\begin{align*}
    2&\dot{x}+\dot{y} -2x= 1 \\ 
    &\dot{x}+\dot{y} -3x -3y= 2, \;\;x(0)=0,\;y(0)=0 
   \end{align*}$$